Finish bulk of `exp_eq` completeness proof
TODO: a few annoying cheats for `Loc`s

meta-theory/pure_ctxt_equivScript.sml
@@ -1,9 +1,11 @@
 
-open HolKernel Parse boolLib bossLib term_tactic;
-open arithmeticTheory listTheory stringTheory alistTheory optionTheory
-     pairTheory pred_setTheory;
-open pure_expTheory pure_exp_lemmasTheory
+open HolKernel Parse boolLib bossLib BasicProvers dep_rewrite;
+open arithmeticTheory listTheory rich_listTheory alistTheory stringTheory
+     optionTheory pairTheory pred_setTheory finite_mapTheory;
+open pure_miscTheory pure_expTheory pure_exp_lemmasTheory
+     pure_evalTheory pure_eval_lemmasTheory pure_semanticsTheory
      pure_exp_relTheory pure_congruenceTheory
+     io_treeTheory pure_obs_sem_equalTheory;
 
 val _ = new_theory "pure_ctxt_equiv";
 
@@ -131,6 +133,501 @@ Proof
     gvs[closed_def] >>
     qspecl_then [`c`,`x`,`y`] assume_tac freevars_plug_eq >> gvs[]
     )
+QED
+
+
+(******************** Contextual equivalence ********************)
+
+Definition ctxt_equiv_def:
+  ctxt_equiv e1 e2 ⇔
+    ∀ctxt. closed (plug ctxt e1) ∧ closed (plug ctxt e2)
+      ⇒ itree_of (plug ctxt e1) = itree_of (plug ctxt e2)
+End
+
+val _ = set_fixity "∽" (Infixl 480);
+Overload "∽" = “ctxt_equiv”;
+
+(******************** Proof apparatus ********************)
+
+Datatype:
+  wh_cons = wh_At lit
+          | wh_Cons string
+          | wh_Clos
+          | wh_Div
+          | wh_Err
+End
+
+Definition wh_to_cons_def:
+  wh_to_cons (wh_Atom a) = wh_At a ∧
+  wh_to_cons (wh_Constructor s es) = wh_Cons s ∧
+  wh_to_cons (wh_Closure x e) = wh_Clos ∧
+  wh_to_cons  wh_Diverge = wh_Div ∧
+  wh_to_cons  wh_Error = wh_Err
+End
+
+Definition step_eval_wh_def:
+  step_eval_wh [] e = SOME (wh_to_cons $ eval_wh e) ∧
+  step_eval_wh (INL (s,n) :: rest) e =
+    (case eval_wh e of
+      wh_Constructor s' es =>
+        if s = s' then OPTION_BIND (oEL n es) (step_eval_wh rest) else NONE
+    | _ => NONE) ∧
+  step_eval_wh (INR arg :: rest) e =
+    case dest_wh_Closure (eval_wh e) of
+      SOME (x, body) =>
+        if closed arg then step_eval_wh rest (subst1 x arg body) else NONE
+    | NONE => NONE
+End
+
+Triviality step_eval_wh_eq:
+  ∀l e1 e2. eval_wh e1 = eval_wh e2 ⇒ step_eval_wh l e1 = step_eval_wh l e2
+Proof
+  Cases >> rw[step_eval_wh_def] >>
+  Cases_on `h` >> rw[step_eval_wh_def] >>
+  PairCases_on `x` >> rw[step_eval_wh_def]
+QED
+
+Triviality app_bisimilarity_wh_to_cons:
+  ∀x y. x ≃ y ⇒ wh_to_cons (eval_wh x) = wh_to_cons (eval_wh y)
+Proof
+  rw[Once app_bisimilarity_iff_alt2] >>
+  Cases_on `eval_wh x` >> gvs[wh_to_cons_def]
+QED
+
+
+(******************** Main lemmas ********************)
+
+Theorem step_eval_wh_IMP_app_similarity[local]:
+  ∀e1 e2.
+    (closed e1 ∧ closed e2 ∧ ∀l. step_eval_wh l e1 = step_eval_wh l e2)
+  ⇒ e1 ≲ e2
+Proof
+  ho_match_mp_tac app_similarity_companion_coind >>
+  rw[FF_def, EXISTS_PROD, unfold_rel_def] >>
+  first_assum (qspec_then `[]` mp_tac) >> simp[step_eval_wh_def] >>
+  Cases_on `eval_wh e2` >> simp[wh_to_cons_def] >> rw[]
+  >- (
+    irule companion_rel >> simp[] >>
+    rpt $ irule_at Any IMP_closed_subst >>
+    simp[IN_FRANGE_FLOOKUP, FLOOKUP_UPDATE] >>
+    imp_res_tac eval_wh_Closure_closed >> simp[] >> rw[] >>
+    rename1 `closed arg` >>
+    first_x_assum $ qspec_then `INR arg :: l` mp_tac >>
+    simp[step_eval_wh_def]
+    ) >>
+  simp[LIST_REL_EL_EQN] >> conj_asm1_tac >> rw[]
+  >- (
+    first_assum $ qspec_then `[INL (s, LENGTH l)]` mp_tac >>
+    first_x_assum $ qspec_then `[INL (s, LENGTH e1s)]` mp_tac >>
+    simp[step_eval_wh_def, oEL_THM]
+    ) >>
+  irule companion_rel >> simp[] >>
+  imp_res_tac eval_wh_freevars_SUBSET >>
+  gvs[closed_def, DISJ_EQ_IMP, MEM_MAP, PULL_FORALL] >>
+  rw[EMPTY_iff_NOTIN] >- metis_tac[EL_MEM] >- metis_tac[EL_MEM] >>
+  rename1 `step_eval_wh ll` >>
+  last_x_assum $ qspec_then `INL (s,n) :: ll` mp_tac >>
+  simp[step_eval_wh_def, oEL_THM]
+QED
+
+Theorem step_eval_wh_eq_app_bisimilarity:
+  ∀e1 e2.
+    closed e1 ∧ closed e2 ∧ (∀l. step_eval_wh l e1 = step_eval_wh l e2) ⇔
+    e1 ≃ e2
+Proof
+  rw[] >> eq_tac
+  >- (
+    rw[app_bisimilarity_similarity] >>
+    irule step_eval_wh_IMP_app_similarity >> simp[]
+    ) >>
+  rw[]
+  >- gvs[Once app_bisimilarity_iff_alt2]
+  >- gvs[Once app_bisimilarity_iff_alt2] >>
+  pop_assum mp_tac >>
+  map_every qid_spec_tac [`e2`,`e1`,`l`] >>
+  Induct >> rw[step_eval_wh_def] >>
+  pop_assum mp_tac >> once_rewrite_tac[app_bisimilarity_iff_alt2] >> strip_tac
+  >- (Cases_on `eval_wh e1` >> gvs[wh_to_cons_def]) >>
+  Cases_on `h` >> gvs[]
+  >- (
+    PairCases_on `x` >> gvs[step_eval_wh_def] >>
+    Cases_on `eval_wh e1` >> gvs[] >> IF_CASES_TAC >> gvs[] >>
+    gvs[oEL_THM, LIST_REL_EL_EQN] >> IF_CASES_TAC >> gvs[]
+    )
+  >- (
+    gvs[step_eval_wh_def] >> Cases_on `eval_wh e1` >> gvs[] >>
+    IF_CASES_TAC >> gvs[]
+    )
+QED
+
+Triviality not_app_bisimilarity_IMP_not_step_eval_wh:
+  ∀e1 e2.
+    ¬ (e1 ≃ e2) ∧ closed e1 ∧ closed e2
+  ⇒ ∃l. step_eval_wh l e1 ≠ step_eval_wh l e2
+Proof
+  rw[] >> CCONTR_TAC >> gvs[] >>
+  drule_all $ iffLR step_eval_wh_eq_app_bisimilarity >> simp[]
+QED
+
+Theorem not_exp_eq_IMP_not_step_eval_wh:
+  ∀e1 e2.
+    ¬ (e1 ≅ e2) ⇒
+    ∃vs es.
+      ALL_DISTINCT vs ∧ EVERY closed es ∧
+      freevars e1 ∪ freevars e2 ⊆ set vs ∧
+      ∃l. step_eval_wh l (Apps (Lams vs e1) es) ≠
+          step_eval_wh l (Apps (Lams vs e2) es)
+Proof
+  rw[exp_eq_def] >> gvs[bind_def] >> EVERY_CASE_TAC >> gvs[] >>
+  qspec_then `f` assume_tac fmap_to_list >> gvs[FDOM_FUPDATE_LIST] >>
+  goal_assum drule >> qexists_tac `MAP SND l` >> simp[] >>
+  conj_asm1_tac
+  >- (
+    gvs[EVERY_MAP, EVERY_MEM, flookup_fupdate_list, alookup_distinct_reverse] >>
+    rw[] >> PairCases_on `x` >> gvs[] >>
+    first_x_assum (qspec_then `x0` assume_tac) >>
+    EVERY_CASE_TAC >> gvs[ALOOKUP_NONE, MEM_MAP] >>
+    drule_all ALOOKUP_ALL_DISTINCT_MEM >> rw[] >> simp[]
+    ) >>
+  drule not_app_bisimilarity_IMP_not_step_eval_wh >> impl_tac
+  >- (
+    rpt $ irule_at Any IMP_closed_subst >> simp[FDOM_FUPDATE_LIST] >>
+    ho_match_mp_tac IN_FRANGE_FUPDATE_LIST_suff >> gvs[EVERY_MEM]
+    ) >>
+  strip_tac >> rename1 `step_eval_wh ll` >> qexists_tac `ll` >>
+  Cases_on `ll` >> gvs[step_eval_wh_def]
+  >- (DEP_REWRITE_TAC[eval_Apps_Lams] >> gvs[EVERY_MAP, combinTheory.o_DEF]) >>
+  reverse $ Cases_on `h` >> gvs[step_eval_wh_def]
+  >- (DEP_REWRITE_TAC[eval_Apps_Lams] >> gvs[EVERY_MAP, combinTheory.o_DEF]) >>
+  reverse $ Cases_on `x` >> gvs[step_eval_wh_def] >>
+  DEP_REWRITE_TAC[eval_Apps_Lams] >> gvs[EVERY_MAP, combinTheory.o_DEF]
+QED
+
+Theorem exists_closed_step_eval_wh:
+  ∀l e1 e2.
+    step_eval_wh l e1 ≠ step_eval_wh l e2
+  ⇒ ∃l'. EVERY (λs. sum_CASE s (K T) closed) l' ∧
+         step_eval_wh l' e1 ≠ step_eval_wh l' e2
+Proof
+  Induct >> rw[step_eval_wh_def]
+  >- (qexists_tac `[]` >> simp[step_eval_wh_def]) >>
+  reverse $ Cases_on `h` >> gvs[step_eval_wh_def]
+  >- (
+    reverse $ EVERY_CASE_TAC >> gvs[]
+    >- (
+      last_x_assum drule >> rw[] >> rename1 `step_eval_wh ll` >>
+      qexists_tac `INR y :: ll` >> simp[step_eval_wh_def]
+      ) >>
+    qexists_tac `[]` >> simp[step_eval_wh_def] >>
+    Cases_on `eval_wh e1` >> gvs[] >>
+    Cases_on `eval_wh e2` >> gvs[wh_to_cons_def]
+    ) >>
+  PairCases_on `x` >>
+  reverse $ Cases_on `step_eval_wh (INL (x0,x1) :: l) e1` >>
+  gvs[step_eval_wh_def]
+  >- (
+    Cases_on `eval_wh e1` >> gvs[oEL_THM] >> rename1 `eval_wh e1 = _ e1s` >>
+    reverse $ Cases_on `∃e2s. eval_wh e2 = wh_Constructor s e2s` >> gvs[]
+    >- (
+      qexists_tac `[]` >> gvs[step_eval_wh_def] >>
+      Cases_on `eval_wh e2` >> gvs[wh_to_cons_def]
+      ) >>
+    last_x_assum (qspecl_then [`EL x1 e1s`,`EL x1 e2s`] assume_tac) >> gvs[] >>
+    Cases_on `x1 < LENGTH e2s` >> gvs[]
+    >- (
+      rename1 `step_eval_wh ll` >>
+      qexists_tac `INL (s,x1) :: ll` >> gvs[step_eval_wh_def, oEL_THM]
+      )
+    >- (qexists_tac `[INL (s,x1)]` >> gvs[step_eval_wh_def, oEL_THM])
+    ) >>
+  Cases_on `eval_wh e2` >> gvs[oEL_THM] >>
+  Cases_on `∃e1s. eval_wh e1 = wh_Constructor s e1s` >> gvs[]
+  >- (qexists_tac `[INL (s,x1)]` >> gvs[step_eval_wh_def, oEL_THM])
+  >- (
+    rename1 `eval_wh e2 = _ e2s` >>
+    last_x_assum $ qspecl_then [`EL x1 e1s`,`EL x1 e2s`] mp_tac >> rw[] >>
+    rename1 `step_eval_wh ll` >>
+    qexists_tac `INL (s,x1) :: ll` >> simp[step_eval_wh_def, oEL_THM]
+    )
+  >- (
+    qexists_tac `[INL (s,x1)]` >> gvs[step_eval_wh_def, oEL_THM] >>
+    Cases_on `eval_wh e1` >> gvs[]
+    )
+QED
+
+Theorem neq_step_eval_IMP_exists_ctxt:
+  ∀l e1 e2.
+    EVERY (λs. sum_CASE s (K T) closed) l ∧
+    closed e1 ∧ closed e2 ∧
+    step_eval_wh l e1 ≠ step_eval_wh l e2
+  ⇒ ∃ctxt.
+      closed (plug ctxt e1) ∧ closed (plug ctxt e2) ∧
+      wh_to_cons (eval_wh $ plug ctxt e1) ≠ wh_to_cons (eval_wh $ plug ctxt e2)
+Proof
+  Induct >> rw[step_eval_wh_def]
+  >- (qexists_tac `Hole` >> simp[plug_def]) >>
+  reverse $ Cases_on `h` >> gvs[step_eval_wh_def]
+  >- (
+    EVERY_CASE_TAC >> gvs[]
+    >- (
+      qexists_tac `Hole` >> simp[plug_def] >>
+      Cases_on `eval_wh e2` >> gvs[] >>
+      Cases_on `eval_wh e1` >> gvs[wh_to_cons_def]
+      )
+    >- (
+      qexists_tac `Hole` >> simp[plug_def] >>
+      Cases_on `eval_wh e1` >> gvs[] >>
+      Cases_on `eval_wh e2` >> gvs[wh_to_cons_def]
+      ) >>
+    last_x_assum $ drule_at $ Pos last >>
+    Cases_on `eval_wh e1` >> gvs[] >> rename1 `eval_wh _ = _ v1 ce1` >>
+    Cases_on `eval_wh e2` >> gvs[] >> rename1 `eval_wh _ = _ v2 ce2` >>
+    impl_keep_tac
+    >- (
+      rpt $ irule_at Any IMP_closed_subst >> simp[FRANGE_FUPDATE] >>
+      imp_res_tac eval_wh_Closure_closed >> gvs[]
+      ) >>
+    rw[] >> qexists_tac `plug_ctxt ctxt (AppL Hole y)` >>
+    simp[plug_plug_ctxt, plug_def] >> simp[CONJ_ASSOC] >> conj_asm1_tac
+    >- (
+      gvs[closed_def] >>
+      qspecl_then [`ctxt`,`App e1 y`,`subst1 v1 y ce1`]
+        assume_tac freevars_plug_eq >> gvs[] >>
+      qspecl_then [`ctxt`,`App e2 y`,`subst1 v2 y ce2`]
+        assume_tac freevars_plug_eq >> gvs[]
+      ) >>
+    `plug ctxt (subst1 v1 y ce1) ≃ plug ctxt (App e1 y) ∧
+     plug ctxt (subst1 v2 y ce2) ≃ plug ctxt (App e2 y)` by (
+      rw[] >> irule app_bisimilarity_plug >> simp[] >> rw[app_bisimilarity_eq] >>
+      irule eval_wh_IMP_exp_eq >> rw[eval_wh_thm, bind1_def]) >>
+    imp_res_tac app_bisimilarity_wh_to_cons >> gvs[]
+    ) >>
+  PairCases_on `x` >>
+  reverse $ Cases_on `step_eval_wh (INL (x0,x1) :: l) e1` >>
+  gvs[step_eval_wh_def]
+  >- (
+    Cases_on `eval_wh e1` >> gvs[oEL_THM] >> rename1 `eval_wh e1 = _ e1s` >>
+    reverse $ Cases_on `∃e2s. eval_wh e2 = wh_Constructor s e2s` >> gvs[]
+    >- (
+      qexists_tac `Hole` >> gvs[plug_def] >>
+      Cases_on `eval_wh e2` >> gvs[wh_to_cons_def]
+      ) >>
+    reverse $ Cases_on `x1 < LENGTH e2s` >> gvs[]
+    >- (
+      rw[] >> qexists_tac `Prim (IsEq s (LENGTH e1s)) [] Hole []` >>
+      simp[plug_def, closed_simps, eval_wh_thm, wh_to_cons_def]
+      ) >>
+    last_x_assum $ qspecl_then [`EL x1 e1s`,`EL x1 e2s`] mp_tac >> gvs[] >>
+    impl_keep_tac
+    >- (
+      imp_res_tac eval_wh_freevars_SUBSET >> gvs[PULL_EXISTS, MEM_MAP] >>
+      gvs[closed_def, EMPTY_iff_NOTIN] >> metis_tac[EL_MEM]
+      ) >>
+    rw[] >> qexists_tac `plug_ctxt ctxt (Prim (Proj s x1) [] Hole [])` >>
+    simp[plug_plug_ctxt, plug_def] >> simp[CONJ_ASSOC] >> conj_asm1_tac
+    >- (
+      gvs[closed_def] >>
+      qspecl_then [`ctxt`,`Proj s x1 e1`,`EL x1 e1s`]
+        assume_tac freevars_plug_eq >> gvs[] >>
+      qspecl_then [`ctxt`,`Proj s x1 e2`,`EL x1 e2s`]
+        assume_tac freevars_plug_eq >> gvs[]
+      ) >>
+    `plug ctxt (EL x1 e1s) ≃ plug ctxt (Proj s x1 e1) ∧
+     plug ctxt (EL x1 e2s) ≃ plug ctxt (Proj s x1 e2)` by (
+      rw[] >> irule app_bisimilarity_plug >> simp[] >> rw[app_bisimilarity_eq] >>
+      irule eval_wh_IMP_exp_eq >> rw[eval_wh_thm]) >>
+    imp_res_tac app_bisimilarity_wh_to_cons >> gvs[]
+    ) >>
+  Cases_on `eval_wh e2` >> gvs[oEL_THM] >> rename1 `eval_wh _ = _ e2s` >>
+  reverse $ Cases_on `∃e1s. eval_wh e1 = wh_Constructor s e1s` >> gvs[]
+  >- (
+    qexists_tac `Prim (IsEq s (LENGTH e2s)) [] Hole []` >>
+    simp[plug_def, eval_wh_thm] >>
+    Cases_on `eval_wh e1` >> gvs[wh_to_cons_def]
+    )
+  >- (
+    qexists_tac `Prim (IsEq s (LENGTH e2s)) [] Hole []` >>
+    simp[plug_def, eval_wh_thm] >>
+    Cases_on `eval_wh e1` >> gvs[wh_to_cons_def]
+    ) >>
+  last_x_assum $ qspecl_then [`EL x1 e1s`,`EL x1 e2s`] mp_tac >> gvs[] >>
+  impl_keep_tac
+  >- (
+    imp_res_tac eval_wh_freevars_SUBSET >> gvs[PULL_EXISTS, MEM_MAP] >>
+    gvs[closed_def, EMPTY_iff_NOTIN] >> metis_tac[EL_MEM]
+    ) >>
+  rw[] >> qexists_tac `plug_ctxt ctxt (Prim (Proj s x1) [] Hole [])` >>
+  simp[plug_plug_ctxt, plug_def] >> simp[CONJ_ASSOC] >> conj_asm1_tac
+  >- (
+    gvs[closed_def] >>
+    qspecl_then [`ctxt`,`Proj s x1 e1`,`EL x1 e1s`]
+      assume_tac freevars_plug_eq >> gvs[] >>
+    qspecl_then [`ctxt`,`Proj s x1 e2`,`EL x1 e2s`]
+      assume_tac freevars_plug_eq >> gvs[]
+    ) >>
+  `plug ctxt (EL x1 e1s) ≃ plug ctxt (Proj s x1 e1) ∧
+   plug ctxt (EL x1 e2s) ≃ plug ctxt (Proj s x1 e2)` by (
+    rw[] >> irule app_bisimilarity_plug >> simp[] >> rw[app_bisimilarity_eq] >>
+    irule eval_wh_IMP_exp_eq >> rw[eval_wh_thm]) >>
+  imp_res_tac app_bisimilarity_wh_to_cons >> gvs[]
+QED
+
+
+(******************** Main theorems ********************)
+
+Theorem exp_eq_eq_ctxt_equiv_lemma:
+  ∀e1 e2.
+    ¬ (e1 ≅ e2)
+  ⇒ ∃ctxt.
+      closed (plug ctxt e1) ∧ closed (plug ctxt e2) ∧
+      wh_to_cons (eval_wh $ plug ctxt e1) ≠ wh_to_cons (eval_wh $ plug ctxt e2)
+Proof
+  rw[] >>
+  imp_res_tac not_exp_eq_IMP_not_step_eval_wh >>
+  imp_res_tac exists_closed_step_eval_wh >>
+  Q.REFINE_EXISTS_TAC `plug_ctxt c (AppLs (LamsC vs Hole) es)` >>
+  simp[plug_plug_ctxt, plug_AppLs, plug_LamsC] >>
+  irule neq_step_eval_IMP_exists_ctxt >> simp[plug_def] >> gvs[UNION_SUBSET] >>
+  goal_assum drule >> simp[]
+QED
+
+Triviality interp_simps[simp]:
+  (∀k st. interp wh_Diverge k st = Ret SilentDivergence) ∧
+  (∀x. interp (wh_Constructor "Ret" [x]) Done [] = Ret Termination) ∧
+  (∀k st. interp wh_Error k st = Ret Error)
+Proof
+  once_rewrite_tac[interp_def] >> simp[next_action_def] >> rw[] >>
+  simp[Once next_def] >> DEEP_INTRO_TAC some_intro >> rw[Once next_def]
+QED
+
+Theorem exp_eq_eq_ctxt_equiv:
+  ∀e1 e2. e1 ≅ e2 ⇔ e1 ∽ e2
+Proof
+  rw[] >> eq_tac >> rw[ctxt_equiv_def]
+  >- (
+    rw[itree_of_def] >>
+    irule bisimilarity_IMP_all_semantics_eq >> simp[] >>
+    rw[app_bisimilarity_eq] >> irule exp_equiv_plug >> simp[]
+    ) >>
+  CCONTR_TAC >> last_x_assum mp_tac >> simp[] >>
+  drule exp_eq_eq_ctxt_equiv_lemma >> rw[] >>
+  Q.REFINE_EXISTS_TAC `plug_ctxt c ctxt` >> simp[plug_plug_ctxt] >>
+  map_every qpat_abbrev_tac [`e1' = plug ctxt e1`, `e2' = plug ctxt e2`] >>
+  Cases_on `eval_wh e1' = wh_Diverge` >> gvs[wh_to_cons_def]
+  >- (
+    `eval_wh e2' ≠ wh_Diverge` by (CCONTR_TAC >> gvs[wh_to_cons_def]) >>
+    qexists_tac `Prim Seq [] Hole [Ret Fail]` >> simp[plug_def] >>
+    simp[itree_of_def, semantics_def, eval_wh_thm] >> IF_CASES_TAC >> gvs[]
+    ) >>
+  Cases_on `eval_wh e2' = wh_Diverge` >> gvs[wh_to_cons_def]
+  >- (
+    qexists_tac `Prim Seq [] Hole [Ret Fail]` >> simp[plug_def] >>
+    simp[itree_of_def, semantics_def, eval_wh_thm] >> IF_CASES_TAC >> gvs[]
+    ) >>
+  Cases_on `eval_wh e1' = wh_Error` >> gvs[wh_to_cons_def]
+  >- (
+    `eval_wh e2' ≠ wh_Error` by (CCONTR_TAC >> gvs[wh_to_cons_def]) >>
+    qexists_tac `Prim Seq [] Hole [Ret Fail]` >> simp[plug_def] >>
+    simp[itree_of_def, semantics_def, eval_wh_thm]
+    ) >>
+  Cases_on `eval_wh e2' = wh_Error` >> gvs[wh_to_cons_def]
+  >- (
+    qexists_tac `Prim Seq [] Hole [Ret Fail]` >> simp[plug_def] >>
+    simp[itree_of_def, semantics_def, eval_wh_thm]
+    ) >>
+  Cases_on `∃s e1s. eval_wh e1' = wh_Constructor s e1s` >> gvs[wh_to_cons_def]
+  >- (
+    qexists_tac
+      `Prim If [] (Prim (IsEq s (LENGTH e1s)) [] Hole []) [Ret Fail; Fail]` >>
+    simp[plug_def, itree_of_def, semantics_def, eval_wh_thm] >>
+    Cases_on `eval_wh e2'` >> gvs[wh_to_cons_def]
+    ) >>
+  Cases_on `∃s e2s. eval_wh e2' = wh_Constructor s e2s` >> gvs[wh_to_cons_def]
+  >- (
+    qexists_tac
+      `Prim If [] (Prim (IsEq s (LENGTH e2s)) [] Hole []) [Ret Fail; Fail]` >>
+    simp[plug_def, itree_of_def, semantics_def, eval_wh_thm] >>
+    Cases_on `eval_wh e1'` >> gvs[wh_to_cons_def]
+    ) >>
+  Cases_on `∃a. eval_wh e1' = wh_Atom a` >> gvs[wh_to_cons_def]
+  >- (
+    Cases_on `a` >> gvs[]
+    >- ( (* Int *)
+      qexists_tac
+        `Prim If [] (Prim (AtomOp Eq) [Lit (Int i)] Hole []) [Ret Fail; Fail]` >>
+      simp[plug_def] >>
+      simp[itree_of_def, semantics_def, eval_wh_thm] >>
+      simp[eval_wh_Prim, pure_evalTheory.get_atoms_def] >>
+      Cases_on `eval_wh e2'` >> gvs[wh_to_cons_def]
+      )
+    >- ( (* Str *)
+      qexists_tac
+        `Prim If [] (Prim (AtomOp Eq) [Lit (Str s)] Hole []) [Ret Fail; Fail]` >>
+      simp[plug_def] >>
+      simp[itree_of_def, semantics_def, eval_wh_thm] >>
+      simp[eval_wh_Prim, pure_evalTheory.get_atoms_def] >>
+      Cases_on `eval_wh e2'` >> gvs[wh_to_cons_def]
+      )
+    >- ( (* Loc *)
+      reverse $ Cases_on `∃m. eval_wh e2' = wh_Atom (Loc m)` >> gvs[]
+      >- cheat (* TODO - allocate n arrays then attempt to access *)
+      >- cheat (* TODO - allocate min (n, m) arrays then attempt to access *)
+      )
+    >- ( (* Msg *)
+      qexists_tac `Prim (Cons "Act") [] Hole []` >> simp[plug_def] >>
+      simp[itree_of_def] >> drule semantics_Act >> strip_tac >> simp[] >>
+      simp[semantics_def, eval_wh_thm] >>
+      once_rewrite_tac[interp_def] >>
+      simp[next_action_def, Once next_def] >>
+      simp[with_atom_def, with_atoms_def] >>
+      Cases_on `eval_wh e2'` >> gvs[get_atoms_def]
+      >- (
+        DEEP_INTRO_TAC some_intro >> rw[Once next_def] >>
+        simp[with_atom_def, with_atoms_def, get_atoms_def, GSYM io_distinct]
+        )
+      >- (
+        simp[AllCaseEqs(), GSYM io_distinct] >> rw[Once next_def] >>
+        simp[with_atom_def, with_atoms_def, get_atoms_def] >>
+        Cases_on `l` >> gvs[wh_to_cons_def]
+        )
+      )
+    ) >>
+  Cases_on `∃a. eval_wh e2' = wh_Atom a` >> gvs[wh_to_cons_def]
+  >- (
+    Cases_on `a` >> gvs[]
+    >- ( (* Int *)
+      qexists_tac
+        `Prim If [] (Prim (AtomOp Eq) [Lit (Int i)] Hole []) [Ret Fail; Fail]` >>
+      simp[plug_def] >>
+      simp[itree_of_def, semantics_def, eval_wh_thm] >>
+      simp[eval_wh_Prim, pure_evalTheory.get_atoms_def] >>
+      Cases_on `eval_wh e1'` >> gvs[wh_to_cons_def]
+      )
+    >- ( (* Str *)
+      qexists_tac
+        `Prim If [] (Prim (AtomOp Eq) [Lit (Str s)] Hole []) [Ret Fail; Fail]` >>
+      simp[plug_def] >>
+      simp[itree_of_def, semantics_def, eval_wh_thm] >>
+      simp[eval_wh_Prim, pure_evalTheory.get_atoms_def] >>
+      Cases_on `eval_wh e1'` >> gvs[wh_to_cons_def]
+      )
+    >- ( (* Loc *)
+      cheat (* TODO - allocate n arrays then attempt to access *)
+      )
+    >- ( (* Msg *)
+      qexists_tac `Prim (Cons "Act") [] Hole []` >> simp[plug_def] >>
+      simp[itree_of_def] >> drule semantics_Act >> strip_tac >> simp[] >>
+      simp[semantics_def, eval_wh_thm] >>
+      once_rewrite_tac[interp_def] >>
+      simp[next_action_def, Once next_def] >>
+      simp[with_atom_def, with_atoms_def] >>
+      Cases_on `eval_wh e1'` >> gvs[get_atoms_def] >>
+      DEEP_INTRO_TAC some_intro >> rw[Once next_def] >>
+      simp[with_atom_def, with_atoms_def, get_atoms_def, GSYM io_distinct]
+      )
+    ) >>
+  Cases_on `eval_wh e1'` >> gvs[] >>
+  Cases_on `eval_wh e2'` >> gvs[wh_to_cons_def]
 QED
 
 
